cleaning up

proof/BigNum_spec.ec
@@ -1,158 +1,155 @@
-require import Core Int IntDiv Ring IntDiv StdOrder List Distr Real.
+require import Core Int IntDiv Ring IntDiv StdOrder List Distr Real DInterval.
 import Ring.IntID IntOrder.
+import StdBigop Bigint BIA.
+
+require import BitEncoding.
+import BS2Int.
 
 require import AuxLemmas.
 
 from Jasmin require import JModel.
 
 require export BigNum_instances.
-
+import W64xN R.
 
 op as_word (x : bool) : W64.t  = x ? W64.one : W64.zero.
 op ith_bitword64 (n : W64.t) (x : int)  : W64.t = as_word (n.[x]).
 
-lemma ones64 : (2^64  - 1)  = 18446744073709551615. smt(). qed.
+lemma ones64 : (2^64  - 1)  = 18446744073709551615. auto. qed.
 op as_bool (x : W64.t) : bool  = (x = W64.one).
 op as_w64 (x : bool) : W64.t  = x ? W64.one : W64.zero.
 
  
 op D : int distr = duniform (range 0 W64xN.modulusR).
 lemma D_ll : is_lossless D. apply duniform_ll.  
- have q : 0 < W64xN.modulusR . smt. smt(@List). qed.
+ have q : 0 < W64xN.modulusR. auto. smt(@List). qed.
 lemma D_uni : is_uniform D. smt(@Distr). qed.
 lemma D_sup x : x \in D <=> 0 <= x < W64xN.modulusR. smt(@Distr). qed.
 lemma D_mu x : x \in D => mu1 D x = Real.inv W64xN.modulusR%r. smt(@Distr). qed.
 
-
 lemma M_pos : 2 < W64xN.modulusR. auto. qed.
 
-op oneR : W64xN.R.t = (W64xN.R.A.of_list W64.zero (W64.one :: nseq (nlimbs - 1) W64.zero)).
 
+(** "Implements" relation *)
+abbrev ImplZZ x y = W64xN.valR x = y.
+  
+op oneR  : W64xN.R.t = W64xN.R.A.of_list W64.zero (W64.one :: nseq (nlimbs - 1) W64.zero).
 op zeroR : W64xN.R.t = W64xN.R.A.of_list W64.zero (List.nseq nlimbs W64.zero).
 
-lemma nseqS' ['a]:
-  forall (n : int) (x : 'a), 0 < n => nseq n x = x :: nseq (n - 1) x.
-smt(nseqS).
-qed.
-
-
 lemma zeroRE: W64xN.valR zeroR = 0.
-proof.
 rewrite /zeroR.
+have nseqS'  : forall  (n : int) (x : W64.t), 0 < n => nseq n x = x :: nseq (n - 1) x. smt(nseqS).
 do? (rewrite nseqS'; first by trivial). simplify.
 rewrite nseq0.
 by rewrite /zeroR W64xN.R.bn2seq /= W64xN.R.A.of_listK 1:/# /bn_seq.
 qed.
 
 
-(** "Implements" relation *)
-abbrev ImplWord x y = W64.to_uint x = y.
-abbrev ImplZZ x y = W64xN.valR x = y.
-abbrev ImplZZ2 x y = W64xN.valR2 x = y.
+lemma oneRE: ImplZZ oneR 1.
+rewrite /oneR /valR /bnk.
+do? (rewrite range_ltn; first by trivial ).
+simplify. rewrite range_geq. auto.
+do rewrite big_consT.
+rewrite big_nil.
+ have -> : W64xN.R.dig ((W64xN.R.A.of_list W64.zero (W64.one :: nseq (nlimbs - 1) W64.zero)))%W64xN.R.A 0 = 1.
+ simplify. smt(@W64 @W64xN.R.A).
+ have q : forall x, 0 < x < nlimbs => W64xN.R.dig ((W64xN.R.A.of_list W64.zero (W64.one :: nseq (nlimbs - 1) W64.zero)))%W64xN.R.A x = 0.
+ move => x xp. rewrite /dig.
+   have ->: to_uint ((W64xN.R.A.of_list W64.zero (W64.one :: nseq (nlimbs - 1) W64.zero)).[x])%A = 0. 
+   have nseqS'  : forall  (n : int) (x : W64.t), 0 < n => nseq n x = x :: nseq (n - 1) x. smt(nseqS).
+    do? (rewrite nseqS'; first by trivial). simplify. 
+   rewrite nseq0.
+  have -> : (A.of_list W64.zero [W64.one; W64.zero]).[x]%A = W64.zero.  
+smt(A.get_of_list). smt().
+smt(@List).  
+do? (rewrite q; first smt()). auto.
+qed.
+
 
 
 module ASpecFp = {
-
   proc addn(a b: int): bool * int = {
     var c, r;
     c <- W64xN.modulusR <= (a+b);
     r <- (a + b) %% W64xN.modulusR;
     return (c, r);
   }
-
   proc daddn(a b: int): bool * int = {
     var c, r;
     c <- W64x2N.modulusR <= (a+b);
     r <- (a + b) %% W64x2N.modulusR;
     return (c, r);
-  }
-  
+  } 
   proc muln(a b: int): int = {
     var r;
     r <- a * b;
     return r;
-  }
-  
+  }  
   proc redm(a p: int): int = {
     var r;
     r <- a %% p;
    return r;
-  }
- 
+  } 
   proc div2(a, n: int): int = {
     var r;
     r <- a %/  (2 ^ n);
    return r;
   }
-
   proc subn(a b: int): bool * int = {
     var c, r;
     c <- a < b;
     r <- (a - b) %% W64xN.modulusR;
     return (c, r);
   }
-
   proc dsubn(a b: int): bool * int = {
     var c, r;
     c <- a < b;
     r <- (a - b) %% W64x2N.modulusR;
     return (c, r);
-  }
-  
+  }  
   proc ctseln(cond: bool, c a: int): int = {
     var r;
     r <- (if cond then a else c);
     return r;
   } 
-
   proc cminus(a p: int): int = {
     var r;
     r <- if a < p then a else a-p;
     return r;
   }
-
   proc rsample(a : int): int = {
     var r;
     r <$ duniform (range 0 a);
     return r;
   }
-
   proc addm(a b p: int): int = {
     var r;
     r <- a + b;
     return r %% p;
-  }
-  
-  
+  }  
 }.
-require import Distr DInterval. 
-require import BitEncoding.
+
 
 module CSpecFp = {
  proc swapr(a : W64xN.R.t, b : W64xN.R.t, c : bool) = {
    return c ? (b,a) : (a, b);
  }
-
  proc ith_bit (r: W64xN.R.t, ctr:int) : W64.t = {
     return (nth false (BS2Int.int2bs (64 * nlimbs) (W64xN.valR r)) ctr) 
               ? W64.one : W64.zero;
  }
-
-
  proc addm(a b p: int): int = {
   var c, x, r;
   (c, x) <@ ASpecFp.addn(a, b);
   r <@ ASpecFp.cminus(x, p);
   return r;
  }
-
  proc daddm(a b p: int): int = {
   var c, x, r;
   (c, x) <@ ASpecFp.daddn(a, b);
   r <@ ASpecFp.cminus(x, p);
   return r;
  }
-
  proc redm(a r k p: int): int = {
    var xr, xrf, xrfn, t, b;
    xr    <@ ASpecFp.muln(a,r);
@@ -163,29 +160,24 @@ module CSpecFp = {
    t     <@ ASpecFp.cminus(t,p);
    return t;
  }
-
  proc cminus(a p: int): int = {
   var c, x, r;
   (c, x) <@ ASpecFp.subn(a, p);
   r <@ ASpecFp.ctseln(c, x, a);
   return r;
  }
-
-
  proc dcminus(a p: int): int = {
   var c, x, r;
   (c, x) <@ ASpecFp.dsubn(a, p);
   r <@ ASpecFp.ctseln(c, x, a);
   return r;
  }
-
  proc mulm(a b p: int): int = {
   var c, z;
   c <@ ASpecFp.muln(a,b);
   z <@ ASpecFp.redm(c,p);
   return z;
  }
-
  proc rsample(a:int) : int * int = {
    var x, b, i,z;
    x <- 0;
@@ -199,7 +191,6 @@ module CSpecFp = {
    }
    return (i,x);
  }
-
 }.
 
 
@@ -210,14 +201,14 @@ proc; simplify.
  inline*. wp. skip.
 progress.
   have ->: (a{2} +  b{2}) %% W64xN.modulusR = (a{2} +  b{2}).
-   rewrite modz_small. split. smt. move => H5. 
-   have ->: `|W64xN.modulusR| = W64xN.modulusR. smt.
-   smt. done.
+   rewrite modz_small. split. smt(). move => H5. 
+   have ->: `|W64xN.modulusR| = W64xN.modulusR. auto. 
+   smt(). done.
   case: (a{2} + b{2} < p{2}) => H5.
    rewrite   modz_small. 
-   smt.
+   smt().
    done.
-   smt.
+   smt().
 qed.
 
 
@@ -228,11 +219,11 @@ proc; simplify.
  inline*. wp. skip.
 progress.
   have ->: (a{2} +  b{2}) %% W64x2N.modulusR = (a{2} +  b{2}).
-   rewrite modz_small. split. smt. move => H5. 
-   have ->: `|W64x2N.modulusR| = W64x2N.modulusR. smt.
-   smt. done.
+   rewrite modz_small. split. smt(). move => H5. 
+   have ->: `|W64x2N.modulusR| = W64x2N.modulusR. auto.
+   smt(). done.
   case: (a{2} + b{2} < p{2}) => H5.
-   rewrite   modz_small. smt. done.
-   smt.
+   rewrite   modz_small. smt(). done.
+   smt().
 qed.
 
